thys/JinjaThreads/Compiler/Compiler1.thy
@@ -17,7 +17,7 @@ where "fresh_var Vs \<equiv> Auxiliary.concat (STR ''V'' # Vs)"
 
 lemma fresh_var_fresh: "fresh_var Vs \<notin> set Vs"
 proof -
-  have "\<forall>V \<in> set Vs. length (explode V) < length (explode (fresh_var Vs))"
+  have "\<forall>V \<in> set Vs. length (String.explode V) < length (String.explode (fresh_var Vs))"
     by(induct Vs)(auto simp add: fresh_var_def Auxiliary.concat_def STR_inverse implode_def)
   thus ?thesis by auto
 qed
